CombinatorLaws.thy
@@ -1,0 +1,120 @@
+theory CombinatorLaws
+imports BananasLanguage
+begin
+
+(* kludged in order to deal with mismatching domains - particularly \<epsilon>*)
+definition expression_equality :: "expr \<Rightarrow> expr \<Rightarrow> bool" (infix "\<simeq>" 50) where
+  "e\<^sub>1 \<simeq> e\<^sub>2 = ((\<forall>v v'. (v ~ e\<^sub>1 \<leadsto> v') \<longrightarrow> (v ~ e\<^sub>2 \<leadsto> v')) \<or> (\<forall>v v'. (v ~ e\<^sub>2 \<leadsto> v') \<longrightarrow> (v ~ e\<^sub>1 \<leadsto> v')))"
+
+(* helper lemmas *)
+
+lemma [elim]: "v ~ (e\<^sub>1 \<cdot> e\<^sub>2) \<cdot> e\<^sub>3 \<leadsto> v' \<Longrightarrow> v ~ e\<^sub>1 \<cdot> e\<^sub>2 \<cdot> e\<^sub>3 \<leadsto> v'"
+  proof (induction v "(e\<^sub>1 \<cdot> e\<^sub>2) \<cdot> e\<^sub>3" v' rule: evaluate.induct)
+  case (ev_comp v v' v'')
+    with ev_comp(3) show ?case 
+      by (induction v' "e\<^sub>1 \<cdot> e\<^sub>2" v'' rule: evaluate.induct) (metis evaluate.ev_comp)
+  qed
+
+lemma [elim]: "v ~ \<epsilon> \<leadsto> v' \<Longrightarrow> v = v'"
+  by (induction v \<epsilon> v' rule: evaluate.induct) simp_all
+
+lemma [elim]: "PairV v\<^sub>1 v\<^sub>2 ~ \<pi>\<^sub>1 \<leadsto> v \<Longrightarrow> v\<^sub>1 = v"
+  by (induction "PairV v\<^sub>1 v\<^sub>2" \<pi>\<^sub>1 v rule: evaluate.induct) simp_all
+
+lemma [elim]: "PairV v\<^sub>1 v\<^sub>2 ~ \<pi>\<^sub>2 \<leadsto> v \<Longrightarrow> v\<^sub>2 = v"
+  by (induction "PairV v\<^sub>1 v\<^sub>2" \<pi>\<^sub>2 v rule: evaluate.induct) simp_all
+
+lemma [elim]: "v ~ \<epsilon> \<cdot> e \<leadsto> v' \<Longrightarrow> v ~ e \<leadsto> v'"
+  proof (induction v "\<epsilon> \<cdot> e" v' rule: evaluate.induct)
+  case (ev_comp v v' v'')
+    moreover hence "v' = v''" by auto
+    ultimately show ?case by simp
+  qed
+
+lemma [elim]: "v ~ e \<cdot> \<epsilon> \<leadsto> v' \<Longrightarrow> v ~ e \<leadsto> v'"
+  proof (induction v "e \<cdot> \<epsilon>" v' rule: evaluate.induct)
+  case (ev_comp v v' v'')
+    moreover hence "v = v'" by auto
+    ultimately show ?case by simp
+  qed
+
+lemma [elim]: "v ~ \<pi>\<^sub>1 \<leadsto> v\<^sub>1 \<Longrightarrow> v ~ \<pi>\<^sub>2 \<leadsto> v\<^sub>2 \<Longrightarrow> v = PairV v\<^sub>1 v\<^sub>2"
+  proof (induction v \<pi>\<^sub>1 v\<^sub>1 rule: evaluate.induct)
+  case (ev_fst v\<^sub>1 v\<^sub>2')
+    thus ?case by (induction "PairV v\<^sub>1 v\<^sub>2'" \<pi>\<^sub>2 v\<^sub>2 rule: evaluate.induct) simp_all
+  qed
+
+lemma [simp]: "v ~ \<pi>\<^sub>1 \<triangle> \<pi>\<^sub>2 \<leadsto> v' \<Longrightarrow> v ~ \<epsilon> \<leadsto> v'"
+  proof (induction v "\<pi>\<^sub>1 \<triangle> \<pi>\<^sub>2" v' rule: evaluate.induct)
+  case (ev_tup v v\<^sub>1 v\<^sub>2)
+    hence "v = PairV v\<^sub>1 v\<^sub>2" by auto
+    thus ?case by simp
+  qed
+
+lemma [simp]: "v ~ e\<^sub>1 \<triangle> e\<^sub>2 \<cdot> e\<^sub>3 \<leadsto> v' \<Longrightarrow> v ~ (e\<^sub>1 \<cdot> e\<^sub>3) \<triangle> (e\<^sub>2 \<cdot> e\<^sub>3) \<leadsto> v'"
+  proof (induction v "e\<^sub>1 \<triangle> e\<^sub>2 \<cdot> e\<^sub>3" v' rule: evaluate.induct)
+  case (ev_comp v v' v'')
+    with ev_comp(3) show ?case by (induction v' "e\<^sub>1 \<triangle> e\<^sub>2" v'' rule: evaluate.induct) simp_all
+  qed
+
+lemma [elim]: "v ~ \<pi>\<^sub>1 \<cdot> e\<^sub>1 \<triangle> e\<^sub>2 \<leadsto> v' \<Longrightarrow> v ~ e\<^sub>1 \<leadsto> v'"
+  proof (induction v "\<pi>\<^sub>1 \<cdot> e\<^sub>1 \<triangle> e\<^sub>2" v' rule: evaluate.induct)
+  case (ev_comp v v' v'')
+    thus ?case 
+      proof (induction v "e\<^sub>1 \<triangle> e\<^sub>2" v' rule: evaluate.induct)
+      case (ev_tup v v\<^sub>1 v\<^sub>2)
+        moreover hence "v\<^sub>1 = v''" by auto
+        ultimately show ?case by simp
+      qed
+  qed
+
+lemma [elim]: "v ~ \<pi>\<^sub>2 \<cdot> e\<^sub>1 \<triangle> e\<^sub>2 \<leadsto> v' \<Longrightarrow> v ~ e\<^sub>2 \<leadsto> v'"
+  proof (induction v "\<pi>\<^sub>2 \<cdot> e\<^sub>1 \<triangle> e\<^sub>2" v' rule: evaluate.induct)
+  case (ev_comp v v' v'')
+    thus ?case 
+      proof (induction v "e\<^sub>1 \<triangle> e\<^sub>2" v' rule: evaluate.induct)
+      case (ev_tup v v\<^sub>1 v\<^sub>2)
+        moreover hence "v\<^sub>2 = v''" by auto
+        ultimately show ?case by simp
+      qed
+  qed
+
+(* in terms of the actual expression equality *)
+
+lemma equiv_refl [simp]: "e\<^sub>1 \<simeq> e\<^sub>1"
+  by (auto simp add: expression_equality_def)
+
+lemma equiv_sym [sym]: "e\<^sub>1 \<simeq> e\<^sub>2 \<Longrightarrow> e\<^sub>2 \<simeq> e\<^sub>1"
+  by (auto simp add: expression_equality_def)
+
+lemma equiv_trans [simp, trans]: "e\<^sub>1 \<simeq> e\<^sub>2 \<Longrightarrow> e\<^sub>2 \<simeq> e\<^sub>3 \<Longrightarrow> e\<^sub>1 \<simeq> e\<^sub>3"
+  by (auto simp add: expression_equality_def)
+
+lemma [simp]: "e\<^sub>1 \<simeq> e\<^sub>2 \<Longrightarrow> e\<^sub>3 \<simeq> e\<^sub>4 \<Longrightarrow> e\<^sub>1 \<cdot> e\<^sub>3 \<simeq> e\<^sub>2 \<cdot> e\<^sub>4"
+  by (auto simp add: expression_equality_def)
+
+lemma [simp]: "e\<^sub>1 \<simeq> e\<^sub>2 \<Longrightarrow> e\<^sub>3 \<simeq> e\<^sub>4 \<Longrightarrow>  e\<^sub>1 \<triangle> e\<^sub>3 \<simeq> e\<^sub>2 \<triangle> e\<^sub>4"
+  by (auto simp add: expression_equality_def)
+
+lemma [simp]: "(e\<^sub>1 \<cdot> e\<^sub>2) \<cdot> e\<^sub>3 \<simeq> e\<^sub>1 \<cdot> e\<^sub>2 \<cdot> e\<^sub>3"
+  by (auto simp add: expression_equality_def)
+
+lemma [simp]: "\<epsilon> \<cdot> e \<simeq> e"
+  by (auto simp add: expression_equality_def)
+
+lemma [simp]: "e \<cdot> \<epsilon> \<simeq> e"
+  by (auto simp add: expression_equality_def)
+
+lemma [simp]: "\<pi>\<^sub>1 \<triangle> \<pi>\<^sub>2 \<simeq> \<epsilon>"
+  by (auto simp add: expression_equality_def)
+
+lemma [simp]: "e\<^sub>1 \<triangle> e\<^sub>2 \<cdot> e\<^sub>3 \<simeq> (e\<^sub>1 \<cdot> e\<^sub>3) \<triangle> (e\<^sub>2 \<cdot> e\<^sub>3)"
+  by (auto simp add: expression_equality_def)
+
+lemma [simp]: "\<pi>\<^sub>1 \<cdot> e\<^sub>1 \<triangle> e\<^sub>2 \<simeq> e\<^sub>1"
+  by (auto simp add: expression_equality_def)
+
+lemma [simp]: "\<pi>\<^sub>2 \<cdot> e\<^sub>1 \<triangle> e\<^sub>2 \<simeq> e\<^sub>2"
+  by (auto simp add: expression_equality_def)
+
+end
